Core/Ty/Definition.lean
@@ -17,16 +17,14 @@ infixr:64 " -:> " => Kind.arrow
 inductive Ty : Type where
 | var : Nat -> Ty
 | global : String -> Ty
-| arrow : BaseKind -> Ty -> Ty -> Ty
+| arrow : Ty -> Ty -> Ty
 | all : Kind -> Ty -> Ty
 | app : Ty -> Ty -> Ty
 | eq : Kind -> Ty -> Ty -> Ty
 
 prefix:max "t#" => Ty.var
 prefix:max "gt#" => Ty.global
-notation A:64 " -[" b "]> " B:65 => Ty.arrow b A B
-infixr:64 " -:> " => Ty.arrow BaseKind.closed
-infixr:64 " =:> " => Ty.arrow BaseKind.open
+infixr:64 " -:> " => Ty.arrow
 notation "∀[" K "]" B => Ty.all K B
 infixl:54 " • " => Ty.app
 notation:55 A:55 " ~[" K "]~ " B => Ty.eq K A B
@@ -42,8 +40,7 @@ instance kindRepr : Repr Kind where
 protected def Ty.repr (p : Nat) : (a : Ty) -> Std.Format
 | var n => "t#" ++ Nat.repr n
 | global s => "gt#" ++ s
-| arrow .closed t1 t2 => Repr.addAppParen (Ty.repr max_prec t1 ++ " -:> " ++ Ty.repr p t2) p
-| arrow .open t1 t2 => Repr.addAppParen (Ty.repr max_prec t1 ++ " =:> " ++ Ty.repr p t2) p
+| arrow t1 t2 => Repr.addAppParen (Ty.repr max_prec t1 ++ " -:> " ++ Ty.repr p t2) p
 | all K t => Repr.addAppParen ("∀[ " ++ repr K ++ " ] " ++ Ty.repr max_prec t) p
 | eq K A B => Repr.addAppParen (Ty.repr max_prec A ++ " ~[" ++ repr K ++ "]~ " ++ Ty.repr max_prec B) p
 | app t1 t2 => Repr.addAppParen (Ty.repr p t1 ++ " • " ++ Ty.repr max_prec t2) p
