Core/Metatheory/Determined.lean
@@ -1,0 +1,104 @@
+import LeanSubst
+import Core.Term
+import Core.Reduction
+import Core.Typing
+
+open LeanSubst
+
+def Term.Determined (t : Term) : Prop :=
+  VariantMissing [.ctor2 .choice, .ctor0 .zero, .guard] t
+
+def Determined.openm (G : List Global) (x : String) : Prop :=
+  ∀ Δ Γ T sp,
+    lookup x G = some (.openm x T) ->
+    sp.length ≥ T.arity ->
+    SpineType x G Δ Γ sp T ->
+    ∃ t, Plus (Red G) ((g#x).apply sp) t ∧ Term.Determined t
+
+def Determined.defn (G : List Global) (x : String) : Prop :=
+  ∀ T t,
+    lookup x G = some (.defn x T t) ->
+    Term.Determined t
+
+def Global.Determined (G : List Global) : Prop :=
+  ∀ x, Determined.openm G x ∧ Determined.defn G x
+
+theorem determined_progress :
+  G&[],[] ⊢ t : A ->
+  t.Determined ->
+  Global.Determined G ->
+  Value G t ∨ (∃ t', Plus (Red G) t t' ∧ t'.Determined)
+:= by
+  sorry
+
+-- Syntactic approximation of determined
+def ExistsUnique {α : Sort u} (p : α → Prop) := ∃ x, p x ∧ ∀ y, p y → y = x
+
+def Trace : Type := List String
+
+inductive InstTrace (G : List Global) : Term -> Trace -> Prop where
+| body : t.Determined -> InstTrace t []
+| lam_open :
+  A.spine = some (x, sp) ->
+  InstTrace t tr ->
+  InstTrace (λ[A] t) tr
+| lam_closed :
+  InstTrace t tr ->
+  InstTrace (λ[A] t) tr
+| guard :
+  InstTrace c tr ->
+  InstTrace (.guard p s c) tr
+
+inductive SpineTrace : List SpineElem -> Trace -> Prop where
+| nil : SpineTrace [] []
+| type : SpineTrace tl tr -> SpineTrace (.type a :: tl) tr
+| term :
+  a.Determined ->
+  SpineTrace tl tr ->
+  SpineTrace (.term a :: tl) tr
+| oterm :
+  a.Determined ->
+  a.spine = some (x, sp) ->
+  SpineTrace tl tr ->
+  SpineTrace (.oterm a :: tl) (x::tr)
+
+def Saturated (G : List Global) : Prop :=
+  ∀ x insts,
+  instances x G = insts ->
+  sorry
+
+theorem inst_red_trace_agree :
+  InstTrace t tr ->
+  SpineTrace sp tr ->
+  G&Δ,Γ ⊢ t.apply sp : T ->
+  ∃ t', Star (Red G) (t.apply sp) t' ∧ t'.Determined
+:= by
+  intro h1 h2 j
+  induction h1 generalizing sp G Δ Γ T
+  case body => sorry
+  case lam t tr b A h1 ih =>
+    cases sp
+    case _ => sorry
+    case _ hd sp =>
+      cases hd
+      case type B =>
+        sorry
+      case term a =>
+        sorry
+      case oterm a =>
+        simp [Term.apply] at *
+        have lem : b = b◯ := sorry -- learned from j
+        subst lem
+        cases h2; case _ x' sp' tr' q1 q2 h2 =>
+
+        sorry
+  case guard =>
+    sorry
+
+theorem inst_red_trace_disagree :
+  InstTrace t tr1 ->
+  SpineTrace sp tr2 ->
+  tr1 ≠ tr2 ->
+  Star (Red G) (t.apply sp) `0
+:= by
+  sorry
