Core/Reduction/Value.lean
@@ -11,189 +11,189 @@ theorem Value.not_zero : ¬ Value G `0 := by
   case _ x sp j1 j2 j3 =>
   simp [Term.spine] at j3
 
-theorem Value.spine_sound :
-  some (x, sp) = t.spine ->
-  (∀ e ∈ sp, ∀ t, .oterm t = e -> ∀ t', ¬ (G ⊢ t ~> t')) ->
-  (∀ e ∈ sp, ∀ t, .oterm t = e -> t.not_choice) ->
-  is_stable x G ∨ OpenVarVal G x sp ->
-  ∀ t', ¬ (G ⊢ t ~> t')
-:= by
-  intro h1 h2 h3 h4 t' r
-  induction sp using List.reverse_ind generalizing x t t'
-  case nil =>
-    have lem := Spine.apply_eq h1
-    rw [lem] at r; simp [Term.apply] at r
-    cases r
-    case inst y sp T tl tl' q1 q2 q3 q4 q5 q6 q7 q8 q9 =>
-      simp [Term.spine] at q8
-      rcases q8 with ⟨e1, e2⟩; subst e1 e2
-      simp at q5
-      cases h4
-      case _ h4 =>
-        unfold is_stable at h4
-        rw [q1] at h4
-        simp at h4
-      case _ h4 =>
-        replace h4 := h4.2 T q4; simp at h4
-        omega
-  case rcons hd tl ih =>
-    cases t <;> try solve | simp [Term.spine] at h1
-    case ctor1 v t =>
-      cases v <;> try solve | simp [Term.spine] at h1
-      case appt =>
-        simp at h1
-        rcases h1 with ⟨sp', e1, e2⟩
-        rcases e1 with ⟨e1, e3⟩; subst e1 e3
-        cases r <;> try solve | simp [Term.spine] at *
-        case inst y sp T tl' tl'' q1 q2 q3 q4 q5 q6 q7 q8 q9 =>
-          simp at q8; rcases q8 with ⟨sp'', e3, e4⟩
-          subst e3; rw [<-e4] at e2; injection e2 with e2
-          injection e2 with e2 e3; subst e2 e3
-          cases h4
-          case _ h4 =>
-            unfold is_stable at h4
-            rw [q1] at h4; simp at h4
-          case _ h4 =>
-            replace h4 := h4.2 T q4
-            simp at h4 q5
-            omega
-        case ctor1_congr t1' _ r =>
-          apply ih e2 _ _ _ _ r
-          case _ =>
-            intro e q1 t q2
-            apply h2 e _ _ q2
-            simp; apply Or.inl q1
-          case _ => sorry
-            -- cases h4
-            -- case _ h4 => apply Or.inl h4
-            -- case _ h4 =>
-            --   apply Or.inr; apply And.intro
-            --   apply h4.1; intro T q
-            --   replace h4 := h4.2 T q
-            --   simp at *; omega
-          case _ =>
-            sorry
-    case ctor2 v t1 t2 =>
-      cases v <;> try solve | simp [Term.spine] at h1
-      case app b =>
-      cases b <;> simp at h1
-      case closed =>
-        rcases h1 with ⟨sp', e1, e2⟩
-        rcases e1 with ⟨e1, e3⟩; subst e1 e3
-        cases r <;> try solve | simp [Term.spine] at *
-        case inst y sp T tl' tl'' q1 q2 q3 q4 q5 q6 q7 q8 q9 =>
-          simp at q8; rcases q8 with ⟨sp'', e3, e4⟩
-          subst e3; rw [<-e4] at e2; injection e2 with e2
-          injection e2 with e2 e3; subst e2 e3
-          cases h4
-          case _ h4 =>
-            unfold is_stable at h4
-            rw [q1] at h4; simp at h4
-          case _ h4 =>
-            replace h4 := h4.2 T q4
-            simp at h4 q5
-            omega
-        case ctor2_congr1 t1' _ r =>
-          apply ih e2 _ _ _ _ r
-          case _ =>
-            intro e q1 t q2
-            apply h2 e _ _ q2
-            simp; apply Or.inl q1
-          case _ =>
-            sorry
-            -- cases h4
-            -- case _ h4 => apply Or.inl h4
-            -- case _ h4 =>
-            --   apply Or.inr; apply And.intro
-            --   apply h4.1; intro T q
-            --   replace h4 := h4.2 T q
-            --   simp at *; omega
-          case _ =>
-            sorry
-      case «open» =>
-        rcases h1 with ⟨sp', e1, e2⟩
-        rcases e1 with ⟨e1, e3⟩; subst e1 e3
-        cases r <;> try solve | simp [Term.spine] at *
-        case inst y sp T tl' tl'' q1 q2 q3 q4 q5 q6 q7 q8 q9 =>
-          simp at q8; rcases q8 with ⟨sp'', e3, e4⟩
-          subst e3; rw [<-e4] at e2; injection e2 with e2
-          injection e2 with e2 e3; subst e2 e3
-          cases h4
-          case _ h4 =>
-            unfold is_stable at h4
-            rw [q1] at h4; simp at h4
-          case _ h4 =>
-            replace h4 := h4.2 T q4
-            simp at h4 q5
-            omega
-        case ctor2_congr1 t1' _ r =>
-          apply ih e2 _ _ _ _ r
-          case _ =>
-            intro e q1 t q2
-            apply h2 e _ _ q2
-            simp; apply Or.inl q1
-          case _ =>
-            sorry
-            -- cases h4
-            -- case _ h4 => apply Or.inl h4
-            -- case _ h4 =>
-            --   apply Or.inr; apply And.intro
-            --   apply h4.1; intro T q
-            --   replace h4 := h4.2 T q
-            --   simp at *; omega
-          case _ =>
-            sorry
-        case ctor2_congr2 t2' _ r =>
+-- theorem Value.spine_sound :
+--   some (x, sp) = t.spine ->
+--   (∀ e ∈ sp, ∀ t, .oterm t = e -> ∀ t', ¬ (G ⊢ t ~> t')) ->
+--   (∀ e ∈ sp, ∀ t, .oterm t = e -> t.not_choice) ->
+--   is_stable x G ∨ OpenVarVal G x sp ->
+--   ∀ t', ¬ (G ⊢ t ~> t')
+-- := by
+--   intro h1 h2 h3 h4 t' r
+--   induction sp using List.reverse_ind generalizing x t t'
+--   case nil =>
+--     have lem := Spine.apply_eq h1
+--     rw [lem] at r; simp [Term.apply] at r
+--     cases r
+--     case inst y sp T tl tl' q1 q2 q3 q4 q5 q6 q7 q8 q9 =>
+--       simp [Term.spine] at q8
+--       rcases q8 with ⟨e1, e2⟩; subst e1 e2
+--       simp at q5
+--       cases h4
+--       case _ h4 =>
+--         unfold is_stable at h4
+--         rw [q1] at h4
+--         simp at h4
+--       case _ h4 =>
+--         replace h4 := h4.2 T q4; simp at h4
+--         omega
+--   case rcons hd tl ih =>
+--     cases t <;> try solve | simp [Term.spine] at h1
+--     case ctor1 v t =>
+--       cases v <;> try solve | simp [Term.spine] at h1
+--       case appt =>
+--         simp at h1
+--         rcases h1 with ⟨sp', e1, e2⟩
+--         rcases e1 with ⟨e1, e3⟩; subst e1 e3
+--         cases r <;> try solve | simp [Term.spine] at *
+--         case inst y sp T tl' tl'' q1 q2 q3 q4 q5 q6 q7 q8 q9 =>
+--           simp at q8; rcases q8 with ⟨sp'', e3, e4⟩
+--           subst e3; rw [<-e4] at e2; injection e2 with e2
+--           injection e2 with e2 e3; subst e2 e3
+--           cases h4
+--           case _ h4 =>
+--             unfold is_stable at h4
+--             rw [q1] at h4; simp at h4
+--           case _ h4 =>
+--             replace h4 := h4.2 T q4
+--             simp at h4 q5
+--             omega
+--         case ctor1_congr t1' _ r =>
+--           apply ih e2 _ _ _ _ r
+--           case _ =>
+--             intro e q1 t q2
+--             apply h2 e _ _ q2
+--             simp; apply Or.inl q1
+--           case _ => sorry
+--             -- cases h4
+--             -- case _ h4 => apply Or.inl h4
+--             -- case _ h4 =>
+--             --   apply Or.inr; apply And.intro
+--             --   apply h4.1; intro T q
+--             --   replace h4 := h4.2 T q
+--             --   simp at *; omega
+--           case _ =>
+--             sorry
+--     case ctor2 v t1 t2 =>
+--       cases v <;> try solve | simp [Term.spine] at h1
+--       case app b =>
+--       cases b <;> simp at h1
+--       case closed =>
+--         rcases h1 with ⟨sp', e1, e2⟩
+--         rcases e1 with ⟨e1, e3⟩; subst e1 e3
+--         cases r <;> try solve | simp [Term.spine] at *
+--         case inst y sp T tl' tl'' q1 q2 q3 q4 q5 q6 q7 q8 q9 =>
+--           simp at q8; rcases q8 with ⟨sp'', e3, e4⟩
+--           subst e3; rw [<-e4] at e2; injection e2 with e2
+--           injection e2 with e2 e3; subst e2 e3
+--           cases h4
+--           case _ h4 =>
+--             unfold is_stable at h4
+--             rw [q1] at h4; simp at h4
+--           case _ h4 =>
+--             replace h4 := h4.2 T q4
+--             simp at h4 q5
+--             omega
+--         case ctor2_congr1 t1' _ r =>
+--           apply ih e2 _ _ _ _ r
+--           case _ =>
+--             intro e q1 t q2
+--             apply h2 e _ _ q2
+--             simp; apply Or.inl q1
+--           case _ =>
+--             sorry
+--             -- cases h4
+--             -- case _ h4 => apply Or.inl h4
+--             -- case _ h4 =>
+--             --   apply Or.inr; apply And.intro
+--             --   apply h4.1; intro T q
+--             --   replace h4 := h4.2 T q
+--             --   simp at *; omega
+--           case _ =>
+--             sorry
+--       case «open» =>
+--         rcases h1 with ⟨sp', e1, e2⟩
+--         rcases e1 with ⟨e1, e3⟩; subst e1 e3
+--         cases r <;> try solve | simp [Term.spine] at *
+--         case inst y sp T tl' tl'' q1 q2 q3 q4 q5 q6 q7 q8 q9 =>
+--           simp at q8; rcases q8 with ⟨sp'', e3, e4⟩
+--           subst e3; rw [<-e4] at e2; injection e2 with e2
+--           injection e2 with e2 e3; subst e2 e3
+--           cases h4
+--           case _ h4 =>
+--             unfold is_stable at h4
+--             rw [q1] at h4; simp at h4
+--           case _ h4 =>
+--             replace h4 := h4.2 T q4
+--             simp at h4 q5
+--             omega
+--         case ctor2_congr1 t1' _ r =>
+--           apply ih e2 _ _ _ _ r
+--           case _ =>
+--             intro e q1 t q2
+--             apply h2 e _ _ q2
+--             simp; apply Or.inl q1
+--           case _ =>
+--             sorry
+--             -- cases h4
+--             -- case _ h4 => apply Or.inl h4
+--             -- case _ h4 =>
+--             --   apply Or.inr; apply And.intro
+--             --   apply h4.1; intro T q
+--             --   replace h4 := h4.2 T q
+--             --   simp at *; omega
+--           case _ =>
+--             sorry
+--         case ctor2_congr2 t2' _ r =>
 
-          sorry
-        case ctor2_absorb2 => sorry
-        case ctor2_map2 c1 c2 _ _ =>
-          replace h3 := h3 (.oterm (c1 `+ c2)) (by simp) (c1 `+ c2) rfl
-          simp [Term.not_choice] at h3
+--           sorry
+--         case ctor2_absorb2 => sorry
+--         case ctor2_map2 c1 c2 _ _ =>
+--           replace h3 := h3 (.oterm (c1 `+ c2)) (by simp) (c1 `+ c2) rfl
+--           simp [Term.not_choice] at h3
 
-theorem Value.sound : Value G t -> ∀ t', ¬ (G ⊢ t ~> t') := by
-  intro j; induction j <;> intro t' r
-  case app x sp t j1 j2 j3 j4 ih =>
-    cases t
-    all_goals try simp [Term.spine] at j1
-    case global y =>
-      rcases j1 with ⟨e1, e2⟩; subst e1 e2
-      cases r; case _ z sp T tl tl' q1 q2 q3 q4 q5 q6 q7 q8 q9 =>
-      simp [Term.spine] at q8
-      rcases q8 with ⟨e1, e2⟩; subst e1 e2; simp at *
-      cases j4
-      case _ j4 =>
-        unfold is_stable at j4
-        exfalso; rw [q1] at j4; simp at j4
-      case _ j4 =>
-        rcases j4 with ⟨j4, j5⟩
-        replace j5 := j5 _ q4; simp at j5
-        rw [q5] at j5; cases j5
-    case ctor1 c t =>
-      cases c <;> try solve | simp [Term.spine] at j1
-      case appt A =>
-        simp at j1
-        rcases j1 with ⟨sp', e1, e2⟩; subst e1
-        apply spine_sound _ ih j3 j4 _ r
-        simp; exact e2
-    case ctor2 c t1 t2 =>
-      cases c <;> try solve | simp [Term.spine] at j1
-      case app b =>
-        cases b
-        case closed =>
-          simp at j1
-          rcases j1 with ⟨sp', e1, e2⟩; subst e1
-          apply spine_sound _ ih j3 j4 _ r
-          simp; exact e2
-        case «open» =>
-          simp at j1
-          rcases j1 with ⟨sp', e1, e2⟩; subst e1
-          apply spine_sound _ ih j3 j4 _ r
-          simp; exact e2
-  case choice t1 t2 j1 j2 ih1 ih2 =>
-    cases r <;> simp at *
-    case inst h _ _ => simp [Term.spine] at h
-    case ctor2_congr1 r _ => apply ih1 _ r
-    case ctor2_congr2 r _ => apply ih2 _ r
-  all_goals
-    cases r <;> simp [Term.spine] at *
+-- theorem Value.sound : Value G t -> ∀ t', ¬ (G ⊢ t ~> t') := by
+--   intro j; induction j <;> intro t' r
+--   case app x sp t j1 j2 j3 j4 ih =>
+--     cases t
+--     all_goals try simp [Term.spine] at j1
+--     case global y =>
+--       rcases j1 with ⟨e1, e2⟩; subst e1 e2
+--       cases r; case _ z sp T tl tl' q1 q2 q3 q4 q5 q6 q7 q8 q9 =>
+--       simp [Term.spine] at q8
+--       rcases q8 with ⟨e1, e2⟩; subst e1 e2; simp at *
+--       cases j4
+--       case _ j4 =>
+--         unfold is_stable at j4
+--         exfalso; rw [q1] at j4; simp at j4
+--       case _ j4 =>
+--         rcases j4 with ⟨j4, j5⟩
+--         replace j5 := j5 _ q4; simp at j5
+--         rw [q5] at j5; cases j5
+--     case ctor1 c t =>
+--       cases c <;> try solve | simp [Term.spine] at j1
+--       case appt A =>
+--         simp at j1
+--         rcases j1 with ⟨sp', e1, e2⟩; subst e1
+--         apply spine_sound _ ih j3 j4 _ r
+--         simp; exact e2
+--     case ctor2 c t1 t2 =>
+--       cases c <;> try solve | simp [Term.spine] at j1
+--       case app b =>
+--         cases b
+--         case closed =>
+--           simp at j1
+--           rcases j1 with ⟨sp', e1, e2⟩; subst e1
+--           apply spine_sound _ ih j3 j4 _ r
+--           simp; exact e2
+--         case «open» =>
+--           simp at j1
+--           rcases j1 with ⟨sp', e1, e2⟩; subst e1
+--           apply spine_sound _ ih j3 j4 _ r
+--           simp; exact e2
+--   case choice t1 t2 j1 j2 ih1 ih2 =>
+--     cases r <;> simp at *
+--     case inst h _ _ => simp [Term.spine] at h
+--     case ctor2_congr1 r _ => apply ih1 _ r
+--     case ctor2_congr2 r _ => apply ih2 _ r
+--   all_goals
+--     cases r <;> simp [Term.spine] at *
