Core/Term/BEq.lean
@@ -47,7 +47,7 @@ def Term.beq : Term -> Term -> Bool
 | ctor1 c1 a1, ctor1 c2 a2 => c1 == c2 && beq a1 a2
 | ctor2 c1 a1 b1, ctor2 c2 a2 b2 => c1 == c2 && beq a1 a2 && beq b1 b2
 | tbind A1 K1 t1, tbind A2 K2 t2 => A1 == A2 && K1 == K2 && beq t1 t2
-| lam b1 A1 t1, lam b2 A2 t2 => b1 == b2 && A1 == A2 && beq t1 t2
+| lam A1 t1, lam A2 t2 => A1 == A2 && beq t1 t2
 | guard a1 b1 c1, guard a2 b2 c2 => beq a1 a2 && beq b1 b2 && beq c1 c2
 | .match (n := n1) a1 ps1 c1, .match (n := n2) a2 ps2 c2 =>
   if h : n1 = n2 then
