Core/Term/Variant.lean
@@ -6,3 +6,66 @@ open LeanSubst
 def Term.not_choice : Term -> Bool
 | ctor2 .choice _ _ => false
 | _ => true
+
+inductive Variant : Type where
+| ctor0 : Ctor0Variant -> Variant
+| ctor1 : Ctor1Variant -> Variant
+| ctor2 : Ctor2Variant -> Variant
+| tbind : TyBindVariant -> Variant
+| lam : Variant
+| guard : Variant
+| mtch : Variant
+
+@[coe]
+def Variant.from_ctor0 (c : Ctor0Variant) : Variant := ctor0 c
+
+instance : Coe Ctor0Variant Variant where
+  coe := Variant.from_ctor0
+
+@[coe]
+def Variant.from_ctor1 (c : Ctor1Variant) : Variant := ctor1 c
+
+instance : Coe Ctor1Variant Variant where
+  coe := Variant.from_ctor1
+
+@[coe]
+def Variant.from_ctor2 (c : Ctor2Variant) : Variant := ctor2 c
+
+instance : Coe Ctor2Variant Variant where
+  coe := Variant.from_ctor2
+
+@[coe]
+def Variant.from_tbind (c : TyBindVariant) : Variant := tbind c
+
+instance : Coe TyBindVariant Variant where
+  coe := Variant.from_tbind
+
+inductive VariantMissing : List Variant -> Term -> Prop where
+| ctor0 {c : Ctor0Variant} :
+  ↑c ∉ vs ->
+  VariantMissing vs (.ctor0 c)
+| ctor1 {c : Ctor1Variant} :
+  ↑c ∉ vs ->
+  VariantMissing vs t ->
+  VariantMissing vs (.ctor1 c t)
+| ctor2 {c : Ctor2Variant} :
+  ↑c ∉ vs ->
+  VariantMissing vs t1 ->
+  VariantMissing vs t2 ->
+  VariantMissing vs (.ctor2 c t1 t2)
+| tbind {c : TyBindVariant} :
+  ↑c ∉ vs ->
+  VariantMissing vs t ->
+  VariantMissing vs (.tbind c K t)
+| lam :
+  VariantMissing vs t ->
+  VariantMissing vs (.lam A t)
+| guard :
+  VariantMissing vs t1 ->
+  VariantMissing vs t2 ->
+  VariantMissing vs t3 ->
+  VariantMissing vs (.guard t1 t2 t3)
+| mtch :
+  VariantMissing vs t ->
+  (∀ i, VariantMissing vs (ts i)) ->
+  VariantMissing vs (.match t ps ts)
