Core/Ty/BEq.lean
@@ -54,7 +54,7 @@ instance instLawfulBeq_Kind : LawfulBEq Kind where
 def Ty.beq : Ty -> Ty -> Bool
 | var x, var y => x == y
 | global x, global y => x == y
-| arrow b1 A1 B1, arrow b2 A2 B2 => b1 == b2 && beq A1 A2 && beq B1 B2
+| arrow A1 B1, arrow A2 B2 => beq A1 A2 && beq B1 B2
 | all K1 P1, all K2 P2 => K1 == K2 && beq P1 P2
 | app A1 B1, app A2 B2 => beq A1 A2 && beq B1 B2
 | eq K1 A1 B1, eq K2 A2 B2 => K1 == K2 && beq A1 A2 && beq B1 B2
